RocqOfRust/revm/revm_interpreter/interpreter_action/simulate/call_inputs.v
@@ -1,0 +1,42 @@
+Require Import simulate.RocqOfRust.
+Require Import alloy_primitives.bytes.links.mod.
+Require Import bytes.links.bytes.
+Require Import core.ops.links.range.
+Require Import revm.revm_interpreter.interpreter_action.links.call_inputs.
+
+Module CallInput.
+  Definition range_len (range : Range.t usize) : usize :=
+    range.(Range.end_) -i range.(Range.start).
+
+  Definition bytes_len (input_bytes : alloy_primitives.bytes.links.mod.Bytes.t) : usize :=
+    {| Integer.value :=
+      Z.of_nat
+        (List.length
+          input_bytes.(alloy_primitives.bytes.links.mod.Bytes.value).(bytes.Bytes.value))
+    |}.
+
+  Definition bytes_as_ref (input_bytes : alloy_primitives.bytes.links.mod.Bytes.t) : list u8 :=
+    input_bytes.(alloy_primitives.bytes.links.mod.Bytes.value).(bytes.Bytes.value).
+
+  Definition len (self : call_inputs.CallInput.t) : usize :=
+    match self with
+    | call_inputs.CallInput.SharedBuffer range => range_len range
+    | call_inputs.CallInput.Bytes bytes => bytes_len bytes
+    end.
+
+  Lemma len_eq
+      (ref_self : '& call_inputs.CallInput.t)
+      (self : call_inputs.CallInput.t)
+      (stack : Stack.t) :
+    CanRead.t stack self ref_self ->
+    {{
+      SimulateM.eval_f
+        (call_inputs.Impl_CallInput.run_len ref_self)
+        stack 🌲
+      (
+        Output.Success (len self),
+        stack
+      )
+    }}.
+  Admitted.
+End CallInput.
